James C - polished up conversion with a bunch of subscripts

TotalCorrectness.thy
@@ -3,31 +3,35 @@ imports AssemblyToMachine StackToAssembly
 begin
 
 definition state_convert :: "stack_program \<Rightarrow> stack_state \<Rightarrow> machine_state set" where
-  "state_convert \<Pi> \<Sigma> = {\<Sigma>'' | \<Sigma>' \<Sigma>''. 
-    \<Sigma>' \<in> StackToAssembly.state_convert \<Sigma> \<and> 
-      \<Sigma>'' \<in> AssemblyToMachine.state_convert (StackToAssembly.program_convert \<Pi>) \<Sigma>'}"
+  "state_convert \<Pi> \<Sigma>\<^sub>S = {\<Sigma>\<^sub>M | \<Sigma>\<^sub>A \<Sigma>\<^sub>M. 
+    \<Sigma>\<^sub>A \<in> StackToAssembly.state_convert \<Sigma>\<^sub>S \<and> 
+      \<Sigma>\<^sub>M \<in> AssemblyToMachine.state_convert (StackToAssembly.program_convert \<Pi>) \<Sigma>\<^sub>A}"
 
 definition program_convert :: "stack_program \<Rightarrow> machine_program" where
   "program_convert \<Pi> = AssemblyToMachine.program_convert (StackToAssembly.program_convert \<Pi>)"
 
-theorem total_correctness: "iterate (eval_stack \<Pi>) \<Sigma> \<Sigma>\<^sub>1 \<Longrightarrow> \<Sigma>' \<in> state_convert \<Pi> \<Sigma> \<Longrightarrow> 
+theorem total_correctness: "iterate (eval_stack \<Pi>) \<Sigma>\<^sub>S \<Sigma>\<^sub>S' \<Longrightarrow> \<Sigma>\<^sub>M \<in> state_convert \<Pi> \<Sigma>\<^sub>S \<Longrightarrow> 
     domain_distinct \<Pi> \<Longrightarrow> 
-      \<exists>\<Sigma>\<^sub>1'. \<Sigma>\<^sub>1' \<in> state_convert \<Pi> \<Sigma>\<^sub>1 \<and> iterate (eval_machine (program_convert \<Pi>)) \<Sigma>' \<Sigma>\<^sub>1'"
+      \<exists>\<Sigma>\<^sub>M'. \<Sigma>\<^sub>M' \<in> state_convert \<Pi> \<Sigma>\<^sub>S' \<and> iterate (eval_machine (program_convert \<Pi>)) \<Sigma>\<^sub>M \<Sigma>\<^sub>M'"
   proof -
-    assume "iterate (eval_stack \<Pi>) \<Sigma> \<Sigma>\<^sub>1"
-    assume "\<Sigma>' \<in> state_convert \<Pi> \<Sigma>"
+    assume "iterate (eval_stack \<Pi>) \<Sigma>\<^sub>S \<Sigma>\<^sub>S'"
     assume "domain_distinct \<Pi>" 
-    
-have "iterate (eval_assembly p\<Pi>) p\<Sigma> p\<Sigma>\<^sub>1 \<Longrightarrow> p\<Sigma>' \<in> AssemblyToMachine.state_convert p\<Pi> p\<Sigma> \<Longrightarrow> 
-  domain_distinct p\<Pi> \<Longrightarrow> 
-    \<exists>\<Sigma>\<^sub>1'. \<Sigma>\<^sub>1' \<in> AssemblyToMachine.state_convert p\<Pi> p\<Sigma>\<^sub>1 \<and> iterate (eval_machine (AssemblyToMachine.program_convert p\<Pi>)) p\<Sigma>' \<Sigma>\<^sub>1'" by (metis assembly_to_machine_correct)
+    assume "\<Sigma>\<^sub>M \<in> state_convert \<Pi> \<Sigma>\<^sub>S"
 
-have "iterate (eval_stack pp\<Pi>) pp\<Sigma> pp\<Sigma>\<^sub>1 \<Longrightarrow> pp\<Sigma>' \<in> StackToAssembly.state_convert pp\<Sigma> \<Longrightarrow> 
-    \<exists>\<Sigma>\<^sub>1'. \<Sigma>\<^sub>1' \<in> StackToAssembly.state_convert pp\<Sigma>\<^sub>1 \<and> iterate (eval_assembly (StackToAssembly.program_convert pp\<Pi>)) pp\<Sigma>' \<Sigma>\<^sub>1'" by (metis stack_to_assembly_correct)
+have "iterate (eval_assembly (StackToAssembly.program_convert \<Pi>)) p\<Sigma> p\<Sigma>\<^sub>1 \<Longrightarrow> p\<Sigma>' \<in> AssemblyToMachine.state_convert (StackToAssembly.program_convert \<Pi>) p\<Sigma> \<Longrightarrow> 
+  domain_distinct (StackToAssembly.program_convert \<Pi>) \<Longrightarrow> 
+    \<exists>\<Sigma>\<^sub>1'. \<Sigma>\<^sub>1' \<in> AssemblyToMachine.state_convert (StackToAssembly.program_convert \<Pi>) p\<Sigma>\<^sub>1 \<and> iterate (eval_machine (AssemblyToMachine.program_convert (StackToAssembly.program_convert \<Pi>))) p\<Sigma>' \<Sigma>\<^sub>1'" by (metis assembly_to_machine_correct)
+
+have "iterate (eval_stack \<Pi>) \<Sigma> \<Sigma>\<^sub>1 \<Longrightarrow> pp\<Sigma>' \<in> StackToAssembly.state_convert \<Sigma> \<Longrightarrow> 
+    \<exists>\<Sigma>\<^sub>1'. \<Sigma>\<^sub>1' \<in> StackToAssembly.state_convert \<Sigma>\<^sub>1 \<and> iterate (eval_assembly (StackToAssembly.program_convert \<Pi>)) pp\<Sigma>' \<Sigma>\<^sub>1'" by (metis stack_to_assembly_correct)
 
 
-    have "\<exists>\<Sigma>\<^sub>1'. \<Sigma>\<^sub>1' \<in> state_convert \<Pi> \<Sigma>\<^sub>1 \<and> iterate (eval_machine (program_convert \<Pi>)) \<Sigma>' \<Sigma>\<^sub>1'" by simp
-    thus ?thesis by simp
+    have "\<Sigma>\<^sub>M' \<in> {\<Sigma>\<^sub>M' | \<Sigma>\<^sub>A' \<Sigma>\<^sub>M'. 
+    \<Sigma>\<^sub>A' \<in> StackToAssembly.state_convert \<Sigma>\<^sub>S' \<and> 
+      \<Sigma>\<^sub>M' \<in> AssemblyToMachine.state_convert (StackToAssembly.program_convert \<Pi>) \<Sigma>\<^sub>A'} \<and> 
+      iterate (eval_machine (AssemblyToMachine.program_convert (StackToAssembly.program_convert \<Pi>))) \<Sigma>\<^sub>M \<Sigma>\<^sub>M'" by simp
+    hence "\<Sigma>\<^sub>M' \<in> state_convert \<Pi> \<Sigma>\<^sub>S' \<and> iterate (eval_machine (program_convert \<Pi>)) \<Sigma>\<^sub>M \<Sigma>\<^sub>M'" by (simp add: state_convert_def program_convert_def)
+    thus ?thesis by fastforce
   qed
 
 end
